fix admits

theories/logrel/big_sepSS.v
@@ -11,7 +11,9 @@ Section definition.
     [∗ set] x1 ∈ s, [∗ set] x2 ∈ s, Φ x1 x2.
 
   Definition big_sepSS_singleton(s : gset K) (x0: K) (Φ : K -> K -> PROP) : PROP:=
-    [∗ set] x∈ s, Φ x0 x ∗ Φ x x0.
+    if decide (x0 ∈ s) then
+    (Φ x0 x0 ∗ ([∗ set] x ∈ (s∖ {[x0]}), Φ x0 x ∗ Φ x x0))%I
+    else ([∗ set] x ∈ (s∖ {[x0]}), Φ x0 x ∗ Φ x x0)%I.
 
   Definition big_sepSS_except(s : gset K) (x0: K) (Φ : K -> K -> PROP) : PROP:=
     big_sepSS (s ∖ {[x0]}) Φ.
@@ -28,23 +30,125 @@ Section lemmas.
     x ∉ s ->
     big_sepSS s Φ ∗ big_sepSS_singleton (s ∪ {[x]}) x Φ ⊢ big_sepSS (s ∪ {[x]}) Φ.
   Proof.
-  Admitted.
+    iIntros (Hnin) "[SS single]".
+    rewrite /big_sepSS.
+    rewrite big_sepS_union.
+    rewrite big_sepS_singleton.
+    rewrite (big_sepS_proper (λ y, [∗ set] x2 ∈ (s ∪ {[x]}), Φ y x2)%I).
+    2:{
+      intros.
+      iApply big_sepS_union.
+      set_solver.
+    }
+    rewrite big_sepS_sep.
+    iFrame "SS".
+    rewrite /big_sepSS_singleton.
+    rewrite 2?big_sepS_union.
+    rewrite 2?big_sepS_singleton.
+    rewrite (big_sepS_proper (λ y, [∗ set] y0 ∈ {[x]}, Φ y y0)%I).
+    2:{
+      intros.
+      iApply big_sepS_singleton.
+    }
+    assert ((s ∪ {[x]}) ∖ {[x]} = s) as ->. set_solver.
+    case_decide.
+    rewrite big_sepS_sep.
+    iDestruct ("single") as "[$ [$ $]]".
+    set_solver.
+    set_solver.
+    set_solver.
+  Qed.
 
   Lemma big_sepSS_difference_singleton s (x0:K) Φ:
     x0 ∈ s ->
     big_sepSS s Φ ⊢ big_sepSS_except s x0 Φ ∗ big_sepSS_singleton s x0 Φ.
   Proof.
-  Admitted.
+    iIntros (Hin) "SS".
+    rewrite /big_sepSS_except /big_sepSS.
+    rewrite /big_sepSS_singleton.
+    assert (s = s ∖ {[x0]} ∪ {[x0]}). rewrite difference_union_L. set_solver + Hin.
+    rewrite H0 in Hin.
+    rewrite H0.
+    assert ((s ∖ {[x0]} ∪ {[x0]}) ∖ {[x0]} = s ∖ {[x0]}) as ->.
+    set_solver +.
+    rewrite big_sepS_union.
+    rewrite big_sepS_singleton.
+    rewrite big_sepS_union.
+    rewrite big_sepS_singleton.
+    rewrite (big_sepS_proper (λ y, [∗ set] x2 ∈ (s ∖ {[x0]} ∪ {[x0]}), Φ y x2)%I).
+    2:{
+      intros.
+      iApply big_sepS_union.
+      set_solver.
+    }
+    rewrite big_sepS_sep.
+    rewrite (big_sepS_proper (λ y, [∗ set] y0 ∈ {[x0]}, Φ y y0)%I).
+    2:{
+      intros.
+      iApply big_sepS_singleton.
+    }
+    case_decide.
+    rewrite big_sepS_sep.
+    iDestruct ("SS") as "(($&$)&$&$)".
+    done.
+    set_solver.
+    set_solver.
+  Qed.
 
   Lemma big_sepSS_sep s Φ Φ1 Φ2 :
-    (∀ x y, Φ x y⊣⊢ Φ1 x y ∗ Φ2 x y) ->
+    (∀ x y, Φ x y ⊣⊢ Φ1 x y ∗ Φ2 x y) ->
     big_sepSS s Φ ⊣⊢ big_sepSS s Φ1 ∗ big_sepSS s Φ2.
   Proof.
-  Admitted.
+    intros.
+    rewrite /big_sepSS.
+    rewrite (big_sepS_proper (λ x1, [∗ set] x2 ∈ s, Φ x1 x2)%I).
+    2:{
+      intros.
+      rewrite (big_sepS_proper (λ x2, Φ x x2)%I).
+      2:{
+        intros.
+        apply H0.
+      }
+      iApply big_sepS_sep.
+    }
+    rewrite big_sepS_sep.
+    done.
+  Qed.
 
   Lemma big_sepSS_singletion_union s v v' Φ :
-    big_sepSS_singleton (s ∖ {[v]}) v' Φ ∗ big_sepSS_singleton {[v]} v' Φ ⊣⊢ big_sepSS_singleton s v' Φ.
+    v ∈ s ->
+    big_sepSS_singleton (s ∖ {[v]}) v' Φ ∗ big_sepSS_singleton {[v]} v' Φ
+    ⊣⊢ big_sepSS_singleton s v' Φ.
   Proof.
-  Admitted.
+    intro.
+    rewrite /big_sepSS_singleton.
+    case_decide.
+    case_decide;first set_solver.
+    case_decide;last set_solver.
+    rewrite -sep_assoc.
+    rewrite -big_sepS_union.
+    rewrite -difference_union_distr_l_L.
+    assert ((s ∖ {[v]} ∪ {[v]}) = s) as ->.
+    rewrite difference_union_L. set_solver.
+    done.
+    set_solver.
+    case_decide.
+    case_decide;last set_solver.
+    rewrite sep_comm .
+    rewrite -sep_assoc.
+    rewrite -big_sepS_union.
+    rewrite -difference_union_distr_l_L.
+    assert (({[v]} ∪ s ∖ {[v]}) = s) as ->.
+    rewrite union_comm_L. rewrite difference_union_L. set_solver.
+    done.
+    set_solver.
+    case_decide. set_solver.
+    rewrite -big_sepS_union.
+    rewrite -difference_union_distr_l_L.
+    assert ((s ∖ {[v]} ∪ {[v]}) = s) as ->.
+    rewrite difference_union_L. set_solver.
+    done.
+    set_solver.
+  Qed.
 
 End lemmas.
